half left for future me

StackMachine.v
@@ -29,3 +29,137 @@ Definition binopDenoteReal : binop -> nat -> nat -> nat :=
 (* CIC enjoys properties like strong normalization and relative consistency *)
 
 (* every Coq source file is a series of vernacular commands, where many command forms take arguments that are Gallina or Ltac programs. *)
+
+Fixpoint expDenote (e : exp) : nat :=
+  match e with
+  | Const n => n
+  | Binop b e1 e2 => (binopDenote b) (expDenote e1) (expDenote e2)
+  end.
+
+(* Unlike with ML, which hardcodes an eager reduction strategy,
+   or Haskell, which hardcodes a lazy strategy,
+   in Coq we are free to choose between these and many other orders of evaluation,
+   because all Coq programs terminate. *)
+
+Eval simpl in expDenote (Const 42).
+Eval simpl in expDenote (Binop Plus (Const 2) (Const 2)).
+Eval simpl in expDenote (Binop Times (Binop Plus (Const 2) (Const 2)) (Const 7)).
+
+Inductive instr : Set :=
+| iConst : nat -> instr
+| iBinop : binop -> instr.
+
+Definition prog := list instr.
+Definition stack := list nat.
+
+Definition instrDenote (i : instr) (s : stack) : option stack :=
+  match i with
+  | iConst n => Some (n :: s)
+  | iBinop b => match s with
+               | arg1 :: arg2 :: s' => Some ((binopDenote b) arg1 arg2 :: s')
+               | _ => None
+               end
+  end.
+
+Fixpoint progDenote (p : prog) (s : stack) : option stack :=
+  match p with
+  | nil => Some s
+  | i :: p' =>
+    match instrDenote i s with
+    | None => None
+    | Some s' => progDenote p' s'
+    end
+  end.
+
+Fixpoint compile (e : exp) : prog :=
+  match e with
+  | Const n => iConst n :: nil
+  | Binop b e1 e2 => compile e2 ++ compile e1 ++ iBinop b :: nil
+  end.
+
+Eval simpl in compile (Const 42).
+Eval simpl in compile (Binop Plus (Const 2) (Const 2)).
+Eval simpl in compile (Binop Times (Binop Plus (Const 2) (Const 2)) (Const 7)).
+
+Lemma compile_correct' : forall e p s,
+    progDenote (compile e ++ p) s = progDenote p (expDenote e :: s).
+Proof.
+  induction e.
+  - intros. unfold expDenote.
+    unfold progDenote at 1. simpl. fold progDenote.
+    reflexivity.
+  (* Hypos are based on term e1 e2 *)
+  - intros.
+    unfold compile. fold compile.
+    unfold expDenote. fold expDenote.
+    rewrite app_assoc_reverse.
+    rewrite IHe2.
+    rewrite app_assoc_reverse.
+    rewrite IHe1.
+    simpl. reflexivity.
+Qed.
+
+Lemma compile_correct'' : forall e s p,
+    progDenote (compile e ++ p) s = progDenote p (expDenote e :: s).
+  induction e; crush.
+Qed.
+
+Theorem compile_correct : forall e,
+    progDenote (compile e) nil = Some (expDenote e :: nil).
+Proof.
+  intro e.
+  rewrite (app_nil_end (compile e)).
+  apply compile_correct'.
+Qed.
+
+(* Coq uses case-sensitive variable names *)
+
+Inductive type : Set :=
+| Nat
+| Bool.
+
+(* We define tbinop as an indexed type family.
+   Indexed inductive types are at the heart of Coq’s expressive power;
+   almost everything else of interest is defined in terms of them *)
+Inductive tbinop : type -> type -> type -> Set :=
+| TPlus : tbinop Nat Nat Nat
+| TTimes : tbinop Nat Nat Nat
+| TEq : forall t, tbinop t t Bool
+| TLt : tbinop Nat Nat Bool.
+
+(* ML and Haskell have indexed algebraic datatypes.
+   For instance, their list types are indexed by the type of data that the list carries.
+   However, compared to Coq, ML and Haskell 98 place two important restrictions on datatype definitions. *)
+
+Inductive texp : type -> Set :=
+| TNConst : nat -> texp Nat
+| TBConst : bool -> texp Bool
+| TBinop : forall t1 t2 t, tbinop t1 t2 t -> texp t1 -> texp t2 -> texp t.
+
+Definition typeDenote (t : type) : Set :=
+  match t with
+  | Nat => nat
+  | Bool => bool
+  end.
+
+
+Definition tbinopDenote arg1 arg2 res (b : tbinop arg1 arg2 res) : typeDenote arg1 -> typeDenote arg2 -> typeDenote res :=
+  match b with
+  | TPlus => plus
+  | TTimes => mult
+  | TEq Nat => beq_nat
+  | TEq Bool => eqb
+  | TLt => leb
+  end.
+
+Fixpoint texpDenote t (e : texp t) : typeDenote t :=
+  match e with
+  | TNConst n => n
+  | TBConst b => b
+  | TBinop _ _ _ b e1 e2 => (tbinopDenote b) (texpDenote e1) (texpDenote e2)
+  end.
+
+Eval simpl in texpDenote (TNConst 42).
+Eval simpl in texpDenote (TBinop TTimes (TBinop TPlus (TNConst 2) (TNConst 2)) (TNConst 7)).
+
+(* I bet first examples are very confused to me ! *)
